MLIR/Dialects/ScfSemantics.lean
@@ -111,7 +111,6 @@ theorem equivalent (b: Bool):
   simp [Semantics.semantics_op, scf_semantics_op]
   simp [interpRegion, denoteRegions]
   simp [run, interpUB_bind, interpSSA'_bind]
-  conv in interpSSA' (Fitree.trigger _) => simp [Fitree.trigger]
   simp [SSAEnvE.handle, cast_eq]
   cases b <;> simp [List.get!]
 
