MLIR/Examples/IfStatementOptimization.lean
@@ -1,0 +1,66 @@
+import MLIR.Dialects.ScfSemantics
+import MLIR.Dialects.ArithSemantics
+open MLIR.AST
+
+namespace SCF_SELECT
+abbrev Δ := scf + arith
+
+def LHS: BasicBlockStmt Δ := [mlir_bb_stmt|
+  %x = "scf.if" (%b) ({
+    "scf.yield"(%n): (i32) -> ()
+  }, {
+    "scf.yield"(%m): (i32) -> ()
+  }): (i1) -> i32
+]
+def RHS: BasicBlockStmt Δ := [mlir_bb_stmt|
+  %x = "select"(%b, %n, %m): (i1, i32, i32) -> i32
+]
+def INPUT (b: FinInt 1) (n m: FinInt 32): SSAEnv Δ := SSAEnv.One [
+  ⟨"b", .i1, b⟩,
+  ⟨"n", .i32, n⟩,
+  ⟨"m", .i32, m⟩]
+
+theorem denoteYieldRegion:
+  denoteRegion Δ (Region.mk
+    [BasicBlock.mk bbname []
+      [BasicBlockStmt.StmtOp
+        (Op.mk "scf.yield" [valuename] [] [] (.mk [])
+          (.fn (.tuple [.int .Signless 32]) (.tuple [])))]]) =
+  fun (args: TypedArgs Δ) =>
+    Fitree.bind (Fitree.trigger <| SSAEnvE.Get MLIRType.i32 valuename) fun x =>
+    Fitree.ret (BlockResult.Ret [⟨.i32, x⟩]) := by
+  funext args
+  simp [denoteRegion, denoteBB, denoteBBStmts, denoteBBStmt, denoteOp]
+  simp [List.zip, List.mapM, List.map]
+  simp [Semantics.semantics_op]
+  simp [HOrElse.hOrElse, OrElse.orElse, Option.orElse, Option.map]
+  simp [scf_semantics_op]
+  simp [denoteTypedArgs]; cases args <;> simp
+
+theorem equivalent (b: FinInt 1) (n m: FinInt 32):
+    (run (denoteBBStmt _ LHS) (INPUT b n m)) =
+    (run (denoteBBStmt _ RHS) (INPUT b n m)) := by
+  simp [LHS, RHS, INPUT]
+  simp [coeMLIRTypeList, coeRegionList, coeBasicBlockStmtList]
+  simp [denoteBBStmt, denoteOp, List.zip, List.mapM, denoteRegions]
+  simp [Semantics.semantics_op]
+  simp [HOrElse.hOrElse, OrElse.orElse, Option.orElse, Option.map]
+  simp [scf_semantics_op, arith_semantics_op]
+  rw [denoteYieldRegion]
+  rw [denoteYieldRegion]
+  save
+
+  conv in Fitree.translate _ (Fitree.trigger _) => simp [Fitree.translate]
+  conv in Fitree.interp (interpRegion Δ) (Fitree.Vis _ _) =>
+    simp [Fitree.interp, interpRegion]
+  simp [run, interpSSA'_bind, SSAEnvE.handle, cast_eq]
+  simp [Fitree.translate]
+  simp [interpRegion, Member.inject, interpSSA'_bind]
+  save
+
+  cases b.bool_cases <;> subst b <;> simp [List.get!, interpSSA'_bind]
+  . simp [Fitree.trigger, Fitree.interp'_bind, SSAEnvE.handle]
+    simp [Fitree.translate, Semantics.handle, cast_eq]
+  . simp [Fitree.trigger, Fitree.interp'_bind, SSAEnvE.handle]
+    simp [Fitree.translate, Semantics.handle, cast_eq]
+end SCF_SELECT
